Foundation/Modal/Kripke/Logic/K4Point2.lean
@@ -46,7 +46,7 @@ instance : Modal.K4 ⪱ Modal.K4Point2 := by
       apply Kripke.not_validOnFrameClass_of_exists_model_world;
       let M : Model := ⟨
         ⟨Fin 2, λ x y => x = 0⟩,
-        λ w a => if a = 0 then True else w = 0
+        λ a w => if a = 0 then True else w = 0
       ⟩;
       use M, 0;
       constructor;
