Foundation/Modal/Kripke/Logic/KT.lean
@@ -54,7 +54,7 @@ instance : Modal.KD ⪱ Modal.KT := by
     . exact axiomT!;
     . apply Sound.not_provable_of_countermodel (𝓜 := FrameClass.KD)
       apply Kripke.not_validOnFrameClass_of_exists_model_world;
-      use ⟨⟨Fin 2, λ x y => y = 1⟩, λ w _ => w = 1⟩, 0;
+      use ⟨⟨Fin 2, λ x y => y = 1⟩, λ _ w => w = 1⟩, 0;
       constructor;
       . exact { serial := by tauto };
       . simp [Semantics.Models, Satisfies];
